cbvlcm: M_heap: finish all proofs

hol_cbvlcm2/M_heapScript.sml
@@ -2,6 +2,7 @@ open HolKernel Parse boolLib bossLib;
 open PrelimsTheory RefinementsTheory LTheory ProgramsTheory;
 open ClosuresTheory M_closTheory CodesTheory;
 open HeapsTheory;
+open relationTheory;
 
 val _ = new_theory "M_heaps";
 
@@ -19,120 +20,328 @@ Section Lin.
   Notation "(≫C_ H )" := (representsClos C H) (at level 0, format "'(≫C_' H ')'").
   Notation "g ≫C_ H e" := (representsClos C H g e) (at level 70,H at level 0, format "g '≫C_' H e").
   Notation "a ≫E_ H E" := (representsEnv C H a E) (at level 70,H at level 0, format "a '≫E_' H E").
+*)
 
-  (* stackStack and Heap *)
-  Definition state := (list HC * list HC *Heap)%type.
+(* stackStack and Heap *)
+Type state = ``:(('a HC) list # ('a HC) list # ('b Heap))``;
 
-  Hint Transparent state.
-
+(* label -> state -> state -> Prop *)
+(* "σ ≻H_ l σ'" := (stepH l σ σ'). *)
+Inductive stepH:
+[~nil:]
+  (∀hImpl C p a T V H.
+    codeImpl.phi C p = SOME retC ⇒
+    stepH hImpl C τ ((p,a)::T,V,H) (T,V,H)) ∧
+[~load:]
+  (∀hImpl C p a x e T V H.
+    codeImpl.phi C p = SOME (varC x) ∧
+    lookup hImpl H a x = SOME e ⇒
+    stepH hImpl C τ ((p,a)::T,V,H) ((codeImpl.inc p,a)::T,e::V,H)) ∧
+[~pushVal:]
+  (∀hImpl C p q a T V H.
+    codeImpl.phi C p = SOME (lamC q) ⇒
+    stepH hImpl C τ ((p,a)::T,V,H) ((codeImpl.inc p,a)::T,(q,a)::V,H)) ∧
+[~beta:]
+  (∀hImpl C a b b' g p q H H' T V.
+    codeImpl.phi C p = SOME (appC) ∧
+    hImpl.put H g b = (H',b') ⇒
+    stepH hImpl C β ((p,a)::T,g::(q,b)::V,H) ((q,b')::(codeImpl.inc p,a)::T,V,H'))
+End
+(*
   Reserved Notation "σ ≻H_ l σ'" (at level 70, l at level 0,format "σ '≻H_' l σ'").
 
-  Inductive stepH : label -> state -> state -> Prop :=
-  | step_nil p a T V H:
-      C p = Some retC ->
-      ((p,a)::T,V,H) ≻H_τ (T,V,H)
-  | step_load p a x e T V H:
-      C p = Some (varC x) ->
-      H.[a,x] = Some e ->
-      ((p,a)::T,V,H) ≻H_τ ((inc p,a)::T,e::V,H)
-  | step_pushVal p q a T V H:
-      C p = Some (lamC q) ->
-      ((p,a)::T,V,H) ≻H_τ ((inc p,a)::T,(q,a)::V,H)
-  | step_beta a b b' g p q H H' T V:
-      C p = Some (appC)
-      -> put H g b = (H',b')
-      -> ((p,a)::T,g::(q,b)::V,H) ≻H_β ((q,b')::(inc p,a)::T,V,H')
-  where "σ ≻H_ l σ'" := (stepH l σ σ').
-
-  Notation "(≻H_ l )" := (stepH l) (at level 0, format "'(≻H_' l ')'").
-  (* workaround to prefere "x ≻ y" over "(≻) x y"*) Notation "σ ≻H_ l σ'" := 0.
+  Notation "(≻H_ l )" := (stepH l) (at level 0, format "'(≻H_' l ')'").*)
+  (* Notation "σ ≻H_ l σ'" := 0.
   Notation "σ ≻H_ l σ'" := (stepH l σ σ').
   Notation "σ ≻H σ'" := (any stepH σ σ') (at level 70).
   Notation "(≻H)" := (any stepH) (at level 0).
 
   Canonical Structure heap_machine := {| M_rel := stepH |}.
+*)
 
-  Hint Constructors stepH.
+(* state -> stateC -> Prop *)
+Inductive repsHC:
+[representsC:]
+  (∀hImpl C H T V T' V'.
+    Forall2 (representsClos hImpl C H) T T' ∧
+    Forall2 (representsClos hImpl C H) V V' ⇒
+    repsHC hImpl C (T,V,H) (T',V'))
+End
 
-  Inductive repsHC : state -> stateC -> Prop :=
-  | representsC H T V T' V': Forall2 (≫C_H) T T' -> Forall2 (≫C_H) V V' -> repsHC (T,V,H) (T',V').
+(*
+Inductive repsHC : state -> stateC -> Prop :=
+| representsC H T V T' V': Forall2 (≫C_H) T T' -> Forall2 (≫C_H) V V' -> repsHC (T,V,H) (T',V').
 
-  Hint Constructors repsHC.
-  Notation "(≫HC)" := (repsHC) (at level 0).
-  Notation "ψ '≫HC' π" := (repsHC ψ π) (at level 70).
+Hint Constructors repsHC.
+Notation "(≫HC)" := (repsHC) (at level 0).
+Notation "ψ '≫HC' π" := (repsHC ψ π) (at level 70).
+*)
 
-  Hint Constructors repsHC.
+Inductive stepC:
+  (∀E T V. stepC (τ: label) (closC retT E::T,V) (T,V)) ∧
+  (∀P E x V p T.
+      nth_error x E = SOME p ⇒
+      stepC τ (closC (varT x P) E::T,V) (closC P E::T,p::V)) ∧
+  (∀P Q E T V.
+      stepC τ (closC (lamT Q P) E ::T,V) (closC P E::T,closC Q E::V)) ∧
+  (∀P E T e Q F V.
+      stepC β (closC (appT P) E :: T,e :: closC Q F ::V) (closC Q (e::F) :: closC P E :: T,V))
+End
 
-  Ltac inv_Mheap :=
-    repeat
-      lazymatch goal with
-      | [H:_ ≫C_ _ _ |-_] => inv H
-      | [H:Forall2 _ (_::_) _ |- _] => inv H
-      | [H:Forall2 _ _ (_::_) |- _] => inv H
-      | [H:Forall2 _ _ [] |- _] => inv H
-      | [H:_ ≫p_ _ _, eq : φ ?C ?a = Some _|- _] =>
-        (inv H;rewrite eq in *;
-         match goal with
-         | [eq' : Some (_)=Some (_) |- _ ] => inv eq'
-            end
-         ;[])
-      | [H:_ ≫p_ _ retT |- _] => inv H
-      | [H:_ ≫p_ _ (lamT _ _) |- _] => inv H
-      | [H:_ ≫p_ _ (varT _ _) |- _] => inv H
-      | [H:_ ≫p_ _ (appT _) |- _] => inv H
-      end.
+Inductive representsClos:
+[~C:]
+  (∀hImpl p a P E.
+    representsPro C p P ∧
+    representsEnv hImpl C H a E ⇒
+    representsClos hImpl C H (p,a) (closC P E))
+End
 
-  Lemma step_simulation π π' ψ l:
-    π ≫HC ψ -> π ≻H_l π' -> exists ψ', π' ≫HC ψ' /\ ψ ≻C_l ψ'.
-  Proof.
-    intros rep R.
-    inv R; inv rep; inv_Mheap.
-    2:edestruct lookup_unlinedEnv with (C:=C) as (?&?&?); [now eassumption..|inv_Mheap].
-    all:eexists;split;[|now eauto 10].
-    all:split;repeat apply Forall2_cons;
-      eauto 8 using Forall2_cons,representsEnv_extend,representsClos_extend,Forall2_impl,HR1,HR2.
-  Qed.
-  Lemma reducible_red π ψ:
-    π ≫HC ψ -> reducible (≻C) ψ -> reducible (≻H) π.
-  Proof.
-    intros rep (ψ'&?&R). inv R; inv rep; inv_Mheap.
-    2:edestruct nth_error_unlinedEnv as (?&?&?);[eassumption..|inv_Mheap].
-    4:edestruct (put H (p,a) a0) eqn:eq.
-    all:now eexists _,_;econstructor; eassumption.
-  Qed.
-  Lemma heap_clos_refinement :
-    refinement_M (≫HC).
-  Proof.
-    split.
-    -apply reducible_red.
-    -eauto using step_simulation.
-  Qed.
-  Lemma compile_heap_clos p a H P:
-    p ≫p_C P ->
-    a ≫E_H [] ->
-    ([(p,a)],[],H) ≫HC ([P/[]],[]).
-  Proof.
-    intros repP repE. eauto.
-  Qed.
+Inductive representsEnv:
+[~Nil:]
+  (∀hImpl C H a. hImpl.get H a = SOME NONE ⇒ representsEnv hImpl C H a []) ∧
+[~Cons:]
+  (∀hImpl C H a b c p P F E.
+         hImpl.get H a = SOME (SOME ((p, b), c)) ∧
+         representsPro C p P ∧
+         representsEnv hImpl C H b F ∧
+         representsEnv hImpl C H c E ⇒
+         representsEnv hImpl C H a ((closC P F)::E))
+End
 
-  Definition repsHL := rcomp (≫HC) (≫CL).
-  Notation "(≫HL)" := (repsHL) (at level 0).
-  Notation "ψ ≫HL s" := (repsHL ψ s) (at level 70).
+Inductive representsPro:
+[~Ret:]
+  (∀p.
+    codeImpl.phi C p = SOME retC ⇒
+    representsPro C p retT) ∧
+[~Var:]
+  (∀p P x.
+    codeImpl.phi C p = SOME (varC x) ∧ representsPro C (codeImpl.inc p) P ⇒
+    representsPro C p (varT x P)) ∧
+[~Lam:]
+  (∀p q P Q.
+    codeImpl.phi C p = SOME (lamC q) ∧ representsPro C (codeImpl.inc p) P ∧
+    representsPro C q Q ⇒
+    representsPro C p (lamT Q P)) ∧
+[~App:]
+  (∀p P.
+    codeImpl.phi C p = SOME appC ∧ representsPro C (codeImpl.inc p) P ⇒
+    representsPro C p (appT P))
+End
 
-  Lemma heap_L_refinement :
-    refinement_ARS (≫HL).
-  Proof.
-    eapply composition;eauto using heap_clos_refinement, clos_L_refinement.
-  Qed.
-  Lemma compile_heap_L p a H s:
-    closedL s ->
-    p ≫p_C γ s retT ->
-    a ≫E_H [] ->
-    ([(p,a)],[],H) ≫HL s.
-  Proof.
-    unfold repsHL in *.
-    intros repP repE. eexists;split.
-    -apply compile_heap_clos. all:eassumption.
-    -apply compile_clos_L. assumption.
-  Qed.
-End Lin.*)
+Theorem step_simulation:
+  ∀hImpl C π π' ψ l.
+    HR hImpl ⇒
+    repsHC hImpl C π ψ ⇒
+    stepH hImpl C l π π' ⇒
+    ∃ψ'. repsHC hImpl C π' ψ' ∧ stepC l ψ ψ'
+Proof
+  rw[] >> PairCases_on `π` >> PairCases_on `ψ` >>
+  PairCases_on `π'` >>
+  qpat_x_assum `repsHC _ _ _ _` mp_tac >>
+  rw[Once repsHC_cases] >>
+  fs[Once stepH_cases] >> rw[] (* 4 *)
+  >- (rw[Once repsHC_cases, PULL_EXISTS] >>
+      qpat_x_assum `Forall2 _ (_::_) _` mp_tac >>
+      rw[Once Forall2_cases] >>
+      qexistsl_tac [`l'`, `ψ1`] >> rw[] >>
+      rw[Once stepC_cases] >>
+      qpat_x_assum `representsClos _ _ _ _ _` mp_tac >>
+      rw[Once representsClos_cases] >>
+      qpat_x_assum `representsPro _ _ _` mp_tac >>
+      rw[Once representsPro_cases])
+  >- (PairCases_on `e`  >>
+      qpat_x_assum `Forall2 _ (_::_) _` mp_tac >>
+      rw[Once Forall2_cases] >>
+      qpat_x_assum `representsClos _ _ _ _ _` mp_tac >>
+      rw[Once representsClos_cases] >>
+      qpat_x_assum `representsPro _ _ _` mp_tac >>
+      rw[Once representsPro_cases] >>
+      drule_all lookup_unlinedEnv >> rw[] >>
+      Cases_on `e` >>
+      rename [`nth_error x E = SOME (closC P E0)`,
+              `representsPro C (codeImpl.inc p) P0`] >>
+      qexists_tac `(closC P0 E :: l', closC P E0 :: ψ1)` >>
+      rw[] (* 2 *)
+      (* repsHC *)
+      >- (rw[Once repsHC_cases] >> (* 2 *)
+          rw[Once Forall2_cases] >>
+          rw[Once representsClos_cases])
+      (* stepC *)
+      >> rw[Once stepC_cases])
+  >- (qpat_x_assum `Forall2 _ (_::_) _` mp_tac >>
+      rw[Once Forall2_cases] >>
+      qpat_x_assum `representsClos _ _ _ _ _` mp_tac >>
+      rw[Once representsClos_cases] >>
+      qpat_x_assum `representsPro _ _ _` mp_tac >>
+      rw[Once representsPro_cases] >>
+      rename [`representsPro C (codeImpl.inc p) P0`] >>
+      qexists_tac `(closC P0 E :: l', closC Q E :: ψ1)` >>
+      rw[] (* 2 *)
+      (* repsHC *)
+      >- (rw[Once repsHC_cases] >> (* 2 *)
+          rw[Once Forall2_cases] >>
+          rw[Once representsClos_cases])
+      (* stepC *)
+      >> rw[Once stepC_cases])
+  >> pop_assum mp_tac >> rw[Once Forall2_cases] >>
+  pop_assum mp_tac >> rw[Once Forall2_cases] >>
+  qpat_x_assum `Forall2 _ (_::_) _` mp_tac >>
+  rw[Once Forall2_cases] >>
+  fs[HR, HR1, HR2] >>
+  first_x_assum drule >> rw[] >>
+  first_x_assum drule >> rw[] >>
+  qpat_x_assum `representsClos hImpl C π2 g y` mp_tac >>
+  rw[Once representsClos_cases] >>
+  rename [`representsPro C p0 P`, `representsEnv hImpl C π2 a0 E`] >>
+  qpat_x_assum `representsClos hImpl C π2 (q,b) y'` mp_tac >>
+  rw[Once representsClos_cases] >>
+  rename [`representsPro C q P0`, `representsEnv hImpl C π2 b E0`] >>
+  qpat_x_assum `representsClos _ _ _ (p,a) _` mp_tac >>
+  rw[Once representsClos_cases] >>
+  rename [`representsPro C p P2`, `representsEnv hImpl C π2 a E1`] >>
+  qpat_x_assum `representsPro C p P2` mp_tac >>
+  rw[Once representsPro_cases] >>
+  rename [`representsPro C (codeImpl.inc p) P2`] >>
+  qexists_tac `(closC P0 (closC P E :: E0) :: (closC P2 E1) :: l', l'')` >>
+  rw[] (* 2 *)
+  (* repsHC *)
+  >- (rw[Once repsHC_cases]
+      >- (rw[Once Forall2_cases]
+          >- (rw[Once representsClos_cases] >>
+              rw[Once representsEnv_cases] >>
+              metis_tac[representsEnv_extend])
+          >> rw[Once Forall2_cases]
+          >- (rw[Once representsClos_cases] >>
+              metis_tac[representsEnv_extend])
+          >> metis_tac[representsClos_extend, Forall2_impl])
+      >> metis_tac[representsClos_extend, Forall2_impl])
+  (* stepC *)
+  >> rw[Once stepC_cases]
+QED
+
+(*
+Lemma step_simulation π π' ψ l:
+  π ≫HC ψ -> π ≻H_l π' -> exists ψ', π' ≫HC ψ' /\ ψ ≻C_l ψ'.
+Proof.
+  intros rep R.
+  inv R; inv rep; inv_Mheap.
+  2:edestruct lookup_unlinedEnv with (C:=C) as (?&?&?); [now eassumption..|inv_Mheap].
+  all:eexists;split;[|now eauto 10].
+  all:split;repeat apply Forall2_cons;
+    eauto 8 using Forall2_cons,representsEnv_extend,representsClos_extend,Forall2_impl,HR1,HR2.
+Qed.
+*)
+
+Theorem reducible_red:
+  ∀hImpl C π ψ.
+    repsHC hImpl C π ψ ⇒
+    reducible (any stepC) ψ ⇒
+    reducible (any (stepH hImpl C)) π
+Proof
+  rw[Once repsHC_cases, Once stepC_cases, Once stepH_cases,
+     reducible, any]
+  >- (qpat_x_assum `Forall2 _ T' _` mp_tac >>
+      rw[Once Forall2_cases] >>
+      qexistsl_tac [`(l,V,H)`, `τ`] >> rw[] >>
+      fs[Once representsClos_cases] >>
+      fs[Once representsPro_cases])
+  >- (qpat_x_assum `Forall2 _ T' _` mp_tac >>
+      rw[Once Forall2_cases] >>
+      fs[Once representsClos_cases] >>
+      fs[Once representsPro_cases] >>
+      metis_tac[nth_error_unlinedEnv])
+  >- (qpat_x_assum `Forall2 _ T' _` mp_tac >>
+      rw[Once Forall2_cases] >>
+      fs[Once representsClos_cases] >>
+      fs[Once representsPro_cases])
+  >> qpat_x_assum `Forall2 _ T' _` mp_tac >>
+  rw[Once Forall2_cases] >>
+  fs[Once representsClos_cases] >>
+  fs[Once representsPro_cases] >>
+  qpat_x_assum `Forall2 _ V _` mp_tac >>
+  rw[Once Forall2_cases] >>
+  qpat_x_assum `Forall2 _ l' _` mp_tac >>
+  rw[Once Forall2_cases] >>
+  PairCases_on `x'` >> rw[] >>
+  Cases_on `hImpl.put H x x'1` >> rw[]
+QED
+
+(*
+Lemma reducible_red π ψ:
+  π ≫HC ψ -> reducible (≻C) ψ -> reducible (≻H) π.
+Proof.
+  intros rep (ψ'&?&R). inv R; inv rep; inv_Mheap.
+  2:edestruct nth_error_unlinedEnv as (?&?&?);[eassumption..|inv_Mheap].
+  4:edestruct (put H (p,a) a0) eqn:eq.
+  all:now eexists _,_;econstructor; eassumption.
+Qed.
+*)
+
+Theorem heap_clos_refinement:
+  HR hImpl ⇒
+  refinement_M (repsHC hImpl C) (stepH hImpl C τ) (stepH hImpl C β) (stepC τ) (stepC β)
+Proof
+  rw[refinement_M]
+  >- (drule reducible_red >> rw[] >>
+      fs[reducible, any, RUNION]
+      >- (`∃x' l. stepH hImpl C l a x'` by metis_tac[] >>
+          Cases_on `l` >> metis_tac[])
+      >> `∃x' l. stepH hImpl C l a x'` by metis_tac[] >>
+      Cases_on `l` >> metis_tac[])
+  >> metis_tac[step_simulation]
+QED
+
+(*
+Lemma heap_clos_refinement :
+  refinement_M (≫HC).
+Proof.
+  split.
+  -apply reducible_red.
+  -eauto using step_simulation.
+Qed.
+*)
+
+Theorem compile_heap_clos:
+  ∀hImpl C p a H P.
+    representsPro C p P ⇒
+    representsEnv hImpl C H a [] ⇒
+    repsHC hImpl C ([(p,a)],[],H) ([closC P []],[])
+Proof
+  rw[repsHC_cases, Once Forall2_cases]
+  >- rw[Once representsClos_cases]
+  >> rw[Once Forall2_cases]
+QED
+
+Definition repsHL:
+  repsHL hImpl C = rcomp (repsHC hImpl C ) repsCL
+End
+
+(*
+Definition repsHL := rcomp (≫HC) (≫CL).
+Notation "(≫HL)" := (repsHL) (at level 0).
+Notation "ψ ≫HL s" := (repsHL ψ s) (at level 70).
+*)
+
+Theorem heap_L_refinement:
+  HR hImpl ⇒
+  refinement_ARS (repsHL hImpl C) (stepH hImpl C τ) (stepH hImpl C β) stepL
+Proof
+  rw[repsHL, rcomp] >>
+  metis_tac[composition, heap_clos_refinement, clos_L_refinement]
+QED
+
+Theorem compile_heap_L:
+  ∀hImpl C p a H s.
+    closedL s ⇒
+    HR hImpl ⇒
+    representsPro C p (gamma s retT) ⇒
+    representsEnv hImpl C H a [] ⇒
+    repsHL hImpl C ([(p,a)],[],H) s
+Proof
+  rw[repsHL, rcomp] >>
+  drule_all compile_heap_clos >> rw[] >>
+  drule compile_clos_L >> rw[] >>
+  metis_tac[]
+QED
+
+val _ = export_theory ()
